examples/compute/src/bir_binpredScript.sml
@@ -1,0 +1,88 @@
+open HolKernel Parse boolLib bossLib
+open bir_basicTheory
+
+
+val _ = new_theory "bir_binpred"
+
+
+(** Gets the operator for a given binary predicate *)
+Definition bir_binpred_get_oper_def:
+    (bir_binpred_get_oper BIExp_Equal = $=) /\
+    (bir_binpred_get_oper BIExp_LessThan = word_lo)
+End
+
+
+(** Evaluates a binary predicate of two immediates *)
+Inductive bir_eval_binpred_imm:
+    (!binpred w1 w2. 
+        bir_eval_binpred_imm binpred (Imm1 w1) (Imm1 w2) ((bir_binpred_get_oper binpred) w1 w2)) /\
+    (!binpred w1 w2. 
+        bir_eval_binpred_imm binpred (Imm8 w1) (Imm8 w2) ((bir_binpred_get_oper binpred) w1 w2)) /\
+    (!binpred w1 w2. 
+        bir_eval_binpred_imm binpred (Imm16 w1) (Imm16 w2) ((bir_binpred_get_oper binpred) w1 w2)) /\
+    (!binpred w1 w2. 
+        bir_eval_binpred_imm binpred (Imm32 w1) (Imm32 w2) ((bir_binpred_get_oper binpred) w1 w2)) /\
+    (!binpred w1 w2. 
+        bir_eval_binpred_imm binpred (Imm64 w1) (Imm64 w2) ((bir_binpred_get_oper binpred) w1 w2)) /\
+    (!binpred w1 w2. 
+        bir_eval_binpred_imm binpred (Imm128 w1) (Imm128 w2) ((bir_binpred_get_oper binpred) w1 w2))
+End
+
+
+(** Evaluates a general binary predicate with values as parameters *)
+Inductive bir_eval_binpred:
+    (!binpred imm1 imm2 b. 
+        (bir_eval_binpred_imm binpred imm1 imm2 b) ==>
+        (bir_eval_binpred binpred (BVal_Imm imm1) (BVal_Imm imm2) (BVal_Imm (bool2b b))))
+End
+
+
+(** ***************** COMPUTE **************** *)
+
+(** Computes a binary predicate of two immediates *)
+Definition bir_compute_binpred_imm_def:
+    (bir_compute_binpred_imm binpred (Imm1 w1) (Imm1 w2) = (bir_binpred_get_oper binpred) w1 w2) /\
+    (bir_compute_binpred_imm binpred (Imm8 w1) (Imm8 w2) = (bir_binpred_get_oper binpred) w1 w2) /\
+    (bir_compute_binpred_imm binpred (Imm16 w1) (Imm16 w2) = (bir_binpred_get_oper binpred) w1 w2) /\
+    (bir_compute_binpred_imm binpred (Imm32 w1) (Imm32 w2) = (bir_binpred_get_oper binpred) w1 w2) /\
+    (bir_compute_binpred_imm binpred (Imm64 w1) (Imm64 w2) = (bir_binpred_get_oper binpred) w1 w2) /\
+    (bir_compute_binpred_imm binpred (Imm128 w1) (Imm128 w2) = (bir_binpred_get_oper binpred) w1 w2) /\
+    (bir_compute_binpred_imm binpred _ _ = F)
+End
+
+
+(** Computes a general binary predicate with values as parameters *)
+Definition bir_compute_binpred_def:
+    (bir_compute_binpred binpred (SOME (BVal_Imm imm1)) (SOME (BVal_Imm imm2)) =
+        SOME (BVal_Imm (bool2b (bir_compute_binpred_imm binpred imm1 imm2)))) /\
+    (bir_compute_binpred _ NONE _ = NONE) /\
+    (bir_compute_binpred _ _ NONE = NONE)
+End
+
+
+
+(* **************** THEOREMS ***************** *)
+Theorem bir_eval_binpred_imp_compute_binpred:
+    !binpred v1 v2 v. bir_eval_binpred binpred v1 v2 v ==> 
+        bir_compute_binpred binpred (SOME v1) (SOME v2) = SOME v
+Proof
+    Cases_on `v1` >> Cases_on `v2` >> Cases_on `v` >>
+        rw [bir_eval_binpred_cases, bir_compute_binpred_def] >>
+        rw [bir_eval_binpred_imm_cases, bir_compute_binpred_imm_def] >>
+        Cases_on `b` >> Cases_on `b'` >>
+            rw [bool2b_def, bool2w_def, bir_compute_binpred_imm_def, bir_imm_t_nchotomy] >>
+            fs [bir_eval_binpred_imm_cases] >>
+            METIS_TAC []
+QED
+
+
+
+
+
+
+
+
+
+
+
+val _ = export_theory ()
